CellularAutomatas/scripts/VerifyConfig.lean
@@ -14,5 +14,30 @@ def verifyConfig : List (Name × List Name) :=
       `Quot.sound,
       `Classical.choice,
       `propext
+    ]),
+    (`CellularAutomatas.proofs.constructions.linear_time_speedup, [
+      `Quot.sound,
+      `Classical.choice,
+      `propext
+    ]),
+    (`CellularAutomatas.proofs.advice_theory.time_advice_combinators, [
+      `Quot.sound,
+      `Classical.choice,
+      `propext
+    ]),
+    (`CellularAutomatas.proofs.advice_theory.compress_n_is_rt_advice, [
+      `Quot.sound,
+      `Classical.choice,
+      `propext
+    ]),
+    (`CellularAutomatas.proofs.advice_theory.run_after_n_time_advice, [
+      `Quot.sound,
+      `Classical.choice,
+      `propext
+    ]),
+    (`CellularAutomatas.proofs.advice_theory.rt_eq_lt_iff_compress2_weak_rt_closed, [
+      `Quot.sound,
+      `Classical.choice,
+      `propext
     ])
   ]
