CellularAutomatas/todo.md
@@ -1,3 +1,0 @@
-# TODO
-
-- [x] Refactor `rt_closed`/`weak_rt_closed` to use `Σ` instead of `∃` (see `refactoring-ideas.md` item 7)
